theories/clang/lib/vmm.v
@@ -1,17 +1,18 @@
 From iris_c.clang Require Import logic notations.
 Require Import iris_c.clang.lib.page_table.
+Require Import iris_c.lib.int.
 
 Section vmm.
   Context `{clangG Σ} {pt: page_table Σ}.
 
   Definition mem_init (n: nat) (x: addr) (y: addr) : expr :=
-    x <- Int.repr 0 ;;
-    while [ !x@Tint32 :<: Int.repr n ] ( !x@Tint32 :<: Int.repr n ) <{
+    x <- 0 ;;
+    while [ !x@Tint32 :<: n ] ( !x@Tint32 :<: n ) <{
       y <- Ealloc (Tprod Tint8 Tvoid) (Vpair vfalse Vvoid) ;;
       Ecall_typed Tvoid (insert_pt pt) [!x@Tint32 ; Evalue (Vptr y)]
     }>.
 
-  Fixpoint allocated m (n: nat) : iProp Σ :=
+  Fixpoint allocated (m: gmap int32 addr) (n: nat) : iProp Σ :=
     match m !! Int.repr n with
       | None => False%I
       | Some p =>
