theories/lib/int.v
@@ -1,0 +1,21 @@
+(* Enhanced Integers *)
+
+Require Export iris_c.lib.Integers.
+Require Import iris.prelude.prelude.
+
+Definition op_safe op (i j: nat) : Prop :=
+    Z.to_nat (Int.intval (op (Int.repr i) (Int.repr j))) = i * j.
+
+Definition mul_safe := op_safe Int.mul.
+
+Coercion Int.repr : Z >-> int32.
+
+Bind Scope int_scope with int.
+Delimit Scope int_scope with int.
+
+Notation "i1 + i2" := (Int.add i1%int i2%int)
+  (at level 50, left associativity) : int_scope.
+Notation "i1 * i2" := (Int.mul i1%int i2%int)
+  (at level 40, left associativity) : int_scope.
+Notation "i1 - i2" := (Int.sub i1%int i2%int)
+  (at level 50, left associativity) : int_scope.
