theories/tests/ret.v
@@ -1,21 +1,15 @@
 From iris_c.clang Require Import notations ret_logic ret_tactics.
+Require Import iris_c.lib.int.
 
 Section example.
   Context `{clangG Σ}.
 
-  Definition one : expr := Int.repr 1.
-
-  Definition ret_one : expr := return: Vint32 (Int.repr 1) ;; return: Vint32 (Int.repr 2).
-
   Lemma one_spec E:
-    True%I ⊢ wpr E one (λ v, ⌜ v = Vint32 (Int.repr 1) ⌝) (λ _, False%I).
+    True%I ⊢ wpr E 1 (λ v, ⌜ v = 1 ⌝) (λ _, False%I).
   Proof. by iApply wpr_value. Qed.
 
   Lemma ret_one_spec E:
-    True%I ⊢ wpr E ret_one (λ _, False%I) (λ v, ⌜ v = Vint32 (Int.repr 1) ⌝).
-  Proof.
-    unfold ret_one. iApply wpr_seq.
-    by iApply wpr_ret.
-  Qed.
+    True%I ⊢ wpr E (return: 1 ;; return: 1) (λ _, False%I) (λ v, ⌜ v = 1 ⌝).
+  Proof. iApply wpr_seq. by iApply wpr_ret. Qed.
 
 End example.
